foldl

src/lists.lean
@@ -1,84 +1,120 @@
-import polyiterate
+import polyfix
 import data.list.basic
+
 
 section list
 
 def ptree_list_encoding_aux : polycodable (list ptree) :=
-{ encode := ⟨ptree.equiv_list.symm, λ x y hxy, by simpa using hxy⟩,
-  mem_poly' := by { convert polydecidable.true, ext x, simp, } }
+{ encode := ptree.equiv_list.symm,
+  decode := ptree.equiv_list,
+  decode_encode := λ _, by simp,
+  polytime_decode := ⟨code.id, polytime_id, by simp⟩}
 
 local attribute [instance] ptree_list_encoding_aux
+
+open polycodable (encode decode)
+open part_eval (with_time eval)
+
 
 lemma encode_list_def (x : list ptree) : polycodable.encode x = ptree.equiv_list.symm x := rfl
 
 lemma polytime_fun.head : polytime_fun (@list.head ptree _) :=
 ⟨code.left, polytime_left,
-by { intro x, dunfold polycodable.encode, cases x; simp, refl, }⟩
+by { intro x, cases x; simp [encode], refl, }⟩
 
 lemma polytime_fun.tail : polytime_fun (@list.tail ptree) :=
 ⟨code.right, polytime_right,
-by { intro x, dunfold polycodable.encode, cases x; simp, }⟩
+by { intro x, cases x; simp [encode], }⟩
 
 lemma polytime_fun.cons : polytime_fun₂ (@list.cons ptree) :=
 ⟨code.id, polytime_id,
-by { intro x, dunfold polycodable.encode, cases x; simp, }⟩
+by { intro x, dunfold polycodable.encode, cases x; simp [encode], }⟩
 
-def foldl_step (f : ptree → ptree → ptree) (x : list ptree × ptree) : list ptree × ptree := (x.1.tail, f x.2 x.1.head)
+variables {α β : Type*} [polycodable α] [polycodable β]
+def foldl_step (f : α → ptree → α) (x : list ptree × α) : option (list ptree × α) :=
+if x.1 = [] then none else some (x.1.tail, f x.2 x.1.head)
 
-lemma polytime_fun.foldl_step {f : ptree → ptree → ptree → ptree} (hf : polytime_fun₃ f) :
+lemma polytime_fun.foldl_step {f : β → α → ptree → α} (hf : polytime_fun₃ f) :
   polytime_fun₂ (λ d, foldl_step (f d)) :=
-by { apply polytime_fun.pair, apply polytime_fun.comp, apply polytime_fun.tail, apply polytime_fun.comp, apply polytime_fun.prod_fst, apply polytime_fun.prod_snd, apply polytime_fun.comp₃ hf, apply polytime_fun.prod_fst, apply polytime_fun.comp, apply polytime_fun.prod_snd, apply polytime_fun.prod_snd, apply polytime_fun.comp, apply polytime_fun.head, apply polytime_fun.comp, apply polytime_fun.prod_fst, apply polytime_fun.prod_snd, }
+by { apply polytime_fun.ite, apply polytime_fun.eq_const, apply polytime_fun.comp polytime_fun.fst polytime_fun.snd, apply polytime_fun.const, apply polytime_fun.comp, apply polytime_fun.some, apply polytime_fun.pair, apply polytime_fun.comp, apply polytime_fun.tail, apply polytime_fun.comp, apply polytime_fun.fst, apply polytime_fun.snd, apply polytime_fun.comp₃ hf, apply polytime_fun.fst, apply polytime_fun.comp, apply polytime_fun.snd, apply polytime_fun.snd, apply polytime_fun.comp, apply polytime_fun.head, apply polytime_fun.comp, apply polytime_fun.fst, apply polytime_fun.snd, }
 
-lemma foldl_step_iterate (f : ptree → ptree → ptree) (i : ℕ) (l : list ptree) (acc : ptree) (hi : i ≤ l.length) :
-  (foldl_step f)^[i] (l, acc) = (l.drop i, (l.take i).foldl f acc) :=
+theorem foldl_step_eval (f : α → ptree → α) (x : list ptree × α) (t : ℕ) :
+  eval (with_time (foldl_step f : list ptree × α →. option (list ptree × α)) (pfun.pure 1)) (t, x) =
+  part.some (t + x.1.length, [], x.1.foldl f x.2) :=
 begin
-  induction i with i ih generalizing acc l, { simp, },
-  cases l with hd tl, { exfalso, simpa using hi, },
-  specialize ih (f acc hd) tl _,
-  { simpa [nat.succ_eq_add_one] using hi, }, { simp [foldl_step, ih], },
+  rcases x with ⟨l, acc⟩, rw [part.eq_some_iff, part_eval.mem_eval],
+  split, swap, { simp [with_time, foldl_step, pfun.pure], },
+  induction l with hd tl ih generalizing acc t, { simp, },
+  have : some (t + 1, tl, f acc hd) ∈ with_time (foldl_step f : list ptree × α →. option (list ptree × α)) (pfun.pure 1) (t, hd :: tl, acc),
+  { simp [with_time, foldl_step, pfun.pure], },
+  refine (part_eval.reaches_fwd this).trans _, simp at ⊢ ih, specialize ih (f acc hd) (t + 1),
+  rw (show (t + (tl.length + 1) = t + 1 + tl.length), by ac_refl), exact ih,
 end
 
-open_locale classical
-noncomputable theory
-
-def foldl_halt (x : list ptree × ptree) := x.1 = []
-
-def foldl_fix_fun (f : ptree → ptree → ptree) := mk_fix_fun_of_iterate (foldl_step f) foldl_halt
-
-lemma polytime_fun.foldl_fix_fun {f : ptree → ptree → ptree → ptree} (hf : polytime_fun₃ f) : polytime_fun₂ (λ d, foldl_fix_fun (f d)) :=
-polytime_fun.mk_fix_fun (polytime_fun.foldl_step hf) (polydecidable_of_preimage_polytime (=[]) polytime_fun.prod_fst $ polydecidable.eq_const _)
-
-
-lemma foldl_fix (f : ptree → ptree → ptree) (l : list ptree) (acc : ptree) :
-  fix_bounded_while (foldl_fix_fun f) (λ x : list ptree × ptree, ∃ i ≤ l.length, l.drop i = x.1 ∧ (l.take i).foldl f acc = x.2) (l.length + 1) (l, acc) = some ([], l.foldl f acc) :=
+theorem foldl_step_eval' (f : α → ptree → α) (x : list ptree × α) :
+  ([], x.1.foldl f x.2) ∈ eval (foldl_step f : list ptree × α →. option (list ptree × α)) x :=
 begin
-  have : nat.iterate (foldl_step f) l.length (l, acc) = ([], l.foldl f acc),
-  { simp [foldl_step_iterate], },
-  convert fix_bounded_while_of_iterate (foldl_step f) foldl_halt (l, acc) l.length _ _,
-  { ext ⟨x₀, x₁⟩, simp [foldl_step_iterate], split,
-    { rintro ⟨i, hi, h₀, h₁⟩, use [i, hi], simp [foldl_step_iterate, hi, h₀, h₁], },
-    rintro ⟨i, hi, h⟩, use [i, hi], simpa [foldl_step_iterate, hi] using h, },
-  { exact this.symm, }, { rw this, simp [foldl_halt], },
-  intros m hm,
-  simpa [foldl_step_iterate, le_of_lt hm, foldl_halt, list.drop_eq_nil_iff_le],
+  have : part_eval.frespects (with_time (foldl_step f : list ptree × α →. option (list ptree × α)) (pfun.pure 1)) (foldl_step f : list ptree × α →. option (list ptree × α)) _ :=
+  part_eval.with_time_respects (by simp [pfun.pure]),
+  have R := foldl_step_eval f x 0, simp [part.eq_some_iff] at R,
+  exact this.of_eval R,
 end
 
-@[simp] lemma encode_sizeof_ptree (x : ptree) : encode_sizeof x = x.sizeof := rfl
-@[simp] lemma encode_sizeof_nil : encode_sizeof ([] : list ptree) = 1 :=
-by { dunfold encode_sizeof, simp [encode_list_def], }
+def foldl_inv (f : α → ptree → α) (x₀ : list ptree × α) : set (list ptree × α) :=
+{s | ∃ i ≤ x₀.1.length, s.1 = x₀.1.drop i ∧ s.2 = (x₀.1.take i).foldl f x₀.2}
+
+theorem foldl_step_invariant (f : α → ptree → α) (x₀) ⦃x y : list ptree × α⦄ (hx : x ∈ foldl_inv f x₀) (hy : some y = foldl_step f x) :
+  y ∈ foldl_inv f x₀ :=
+begin 
+  rcases x with ⟨x₁, x₂⟩, rcases x₀ with ⟨l₀, acc₀⟩,
+  simp [foldl_inv] at hx ⊢,
+  rcases hx with ⟨i, H, rfl, rfl⟩,
+  by_cases l₀.length ≤ i,
+  { simp [h, foldl_step] at hy, contradiction, },
+  simp [foldl_step, list.drop_eq_nil_iff_le, h] at hy,
+  refine ⟨i+1, _, _, _⟩,
+  { rwa [nat.succ_le_iff, lt_iff_not_le], },
+  { rw hy, simp [← list.drop_one], congr' 1, ac_refl, },
+  rw hy, 
+  suffices : l₀.take (i+1) = l₀.take i ++ [(l₀.drop i).head], { simp [this], }, 
+  rw not_le at h,
+  rw [list.drop_eq_nth_le_cons h, list.take_succ, list.nth_le_nth h], simp [option.to_list],
+end
+
+theorem foldl_step_eval_inv (f : α → ptree → α) (x : list ptree × α) :
+  x.1.length + 1 ∈ part_eval.time_iter (pfun.res (foldl_step f) (foldl_inv f x)) (pfun.pure 1) x :=
+begin
+  rw [← pfun.coe_res_inter, ← part_eval.time_iter_invariant],
+  { simp [part_eval.time_iter, pfun.pure, add_comm x.fst.length 1],
+    use [[], x.1.foldl f x.2], rw ← part.eq_some_iff, convert foldl_step_eval f x 0, simp, },
+  { simpa using foldl_step_invariant f x, },
+  use 0, simp,
+end
+
+section encode_sizeof
+
+
+open polycodable (encode)
+
+@[simp] lemma encode_sizeof_ptree (x : ptree) : (encode x).sizeof = x.sizeof := rfl
+@[simp] lemma encode_sizeof_nil : (encode ([] : list ptree)).sizeof = 1 :=
+by simp [encode]
 @[simp] lemma encode_sizeof_cons (a : ptree) (b : list ptree) :
-  encode_sizeof (a :: b) = 1 + encode_sizeof a + encode_sizeof b :=
-by { dunfold encode_sizeof, simp [encode_list_def], }
-lemma one_le_encode_sizeof {α : Type*} [polycodable α] (x : α) :
-  1 ≤ encode_sizeof x :=
-by { dunfold encode_sizeof, cases (polycodable.encode x); simp, linarith, }
+  (encode (a :: b)).sizeof = 1 + (encode a).sizeof + (encode b).sizeof :=
+by simp [encode]
+lemma one_le_encode_sizeof (x : α) :
+  1 ≤ (encode x).sizeof :=
+by { cases (encode x); simp, linarith only, }
+
+@[simp] lemma encode_sizeof_pair (a : α) (b : β) : (encode (a, b)).sizeof = (encode a).sizeof + (encode b).sizeof + 1 :=
+by { simp [encode], ac_refl, }
 
 @[simp] lemma encode_sizeof_append (a b : list ptree) :
-  (encode_sizeof (a ++ b) : ℤ) = ((encode_sizeof a) : ℤ) + (encode_sizeof b) - 1 :=
+  ((encode (a ++ b)).sizeof : ℤ) = ((encode a).sizeof : ℤ) + (encode b).sizeof - 1 :=
 by { induction a with hd tl ih, { simp, }, simp [ih], ring, }
 
 lemma encode_sizeof_le_of_infix {a b : list ptree} (h : a <:+: b) :
-  encode_sizeof a ≤ encode_sizeof b :=
+  (encode a).sizeof ≤ (encode b).sizeof :=
 begin
   rcases h with ⟨s, t, rfl⟩,
   have i₁ := one_le_encode_sizeof s, have i₂ := one_le_encode_sizeof t,
@@ -86,99 +122,47 @@ begin
 end
 
 lemma len_le_encode_sizeof (a : list ptree) :
-  a.length + 1 ≤ encode_sizeof a :=
+  a.length + 1 ≤ (encode a).sizeof :=
 by { induction a with hd tl ih, { simp, }, simp, linarith, }
 
-def polysize_fun {α β : Type*} [polycodable α] [polycodable β] (f : α → β) : Prop :=
-∃ p : polynomial ℕ, ∀ (n : ℕ) (x : α), encode_sizeof x ≤ n → encode_sizeof (f x) ≤ p.eval n
 
-lemma polysize_of_polytime_fun {α β : Type*} [polycodable α] [polycodable β] (f : α → β) (hf : polytime_fun f) :
+def polysize_fun (f : α → β) : Prop :=
+∃ p : polynomial ℕ, ∀ (x : α), (encode (f x)).sizeof ≤ p.eval (encode x).sizeof
+
+lemma polysize_of_polytime_fun (f : α → β) (hf : polytime_fun f) :
   polysize_fun f :=
 begin
-  obtain ⟨c, ⟨p, hp⟩, s⟩ := hf, use p, intros n x hx,
-  obtain ⟨t, ht₀, ht₁⟩ := hp n (polycodable.encode x) hx,
-  specialize s x, rw part.eq_some_iff at s,
-  exact (eval_sizeof_le_time s ht₀).trans ht₁,
+  rcases hf with ⟨c, ⟨p, hp⟩, sc⟩, use p,
+  intro x, specialize sc x, rw part.eq_some_iff at sc,
+  rcases hp (encode x) with ⟨t, ht, t_le⟩,
+  exact (eval_sizeof_le_time sc ht).trans t_le,
 end
 
+end encode_sizeof
 
-lemma polytime_fun.foldl' {f : ptree → ptree → ptree → ptree} {g : ptree → list ptree} {acc : ptree → ptree}
-  (hf : polytime_fun₃ f) (hg : polytime_fun g) (hacc : polytime_fun acc) 
-  (hsize : polysize_fun (λ xls : list ptree × ptree × ptree, xls.1.foldl (f xls.2.1) xls.2.2)) :
-  polytime_fun (λ x, (@list.nil ptree, (g x).foldl (f x) (acc x))) :=
+theorem polytime_fun.foldl (f : β → α → ptree → α) (l : β → list ptree) (acc : β → α) 
+  (hf : polytime_fun₃ f) (hl : polytime_fun l) (hacc : polytime_fun acc) 
+  (hs : polysize_fun (λ xls : β × α × list ptree, xls.2.2.foldl (f xls.1) xls.2.1)) :
+  polytime_fun (λ s, (l s).foldl (f s) (acc s)) :=
 begin
-  cases hsize with q hq,
-  have := polytime_fix_bounded' (polynomial.monomial 1 1) (q + polynomial.monomial 1 1)
-    (λ d, foldl_fix_fun (f d)) (λ d x, ([], x.1.foldl (f d) x.2)) _ _,
-  { have := polytime_fun.comp₂ this polytime_fun.id (polytime_fun.pair hg hacc), exact this, },
-  { rintros d ⟨l, s⟩, dsimp only,
-    apply fix_bounded_while_weaken _ _ (foldl_fix (f d) l s),
-    { rintros ⟨l', s'⟩, dsimp only, rintros ⟨i, H, rfl, rfl⟩, 
-      specialize hq _ ⟨l.take i, d, s⟩ rfl.le, dsimp only at hq,
-      simp, conv_rhs { rw [add_comm, add_assoc], }, apply le_add_of_nonneg_of_le, { exact zero_le', },
-      mono,
-      { linarith only [encode_sizeof_le_of_infix (l.drop_suffix i).is_infix], },
-      refine hq.trans _, apply monotone_polynomial_nat, simp, linarith only [encode_sizeof_le_of_infix (l.take_prefix i).is_infix], },
-    refine (len_le_encode_sizeof _).trans _, simp, linarith only, },
-  { apply polytime_fun.foldl_fix_fun hf, }
+  suffices : polytime_fun₃ (λ s (L : list ptree) (a : α), (@list.nil ptree, L.foldl (f s) a)),
+  { have pf : polytime_fun (λ s, (s, l s, acc s)) := polytime_fun.pair polytime_fun.id (polytime_fun.pair hl hacc),
+    exact polytime_fun.comp polytime_fun.snd (polytime_fun.comp this pf), },
+  cases hs with ps hps,
+  refine polytime_fun.eval (λ s : β, foldl_step (f s)) (λ (s : β) (x : list ptree × α), ([], x.1.foldl (f s) x.2))
+    _ (polynomial.monomial 1 1) (ps + polynomial.monomial 1 1) _ _,
+  { exact polytime_fun.foldl_step hf, },
+  { rintros s ⟨l₀, a₀⟩, simp, apply foldl_step_eval', },
+  rintros S ⟨l₀, a₀⟩, use l₀.length + 1, split,
+  { simp, linarith only [len_le_encode_sizeof l₀], },
+  apply part_eval.time_iter_mono _ (foldl_step_eval_inv (f S) (l₀, a₀)),
+  rintros ⟨l₁, a₁⟩ y, simp [pfun.mem_res], rintros h₁ h₂, refine ⟨_, h₂⟩,
+  simp [foldl_inv] at h₁, rcases h₁ with ⟨i, hi, rfl, rfl⟩,
+  ring_nf, simp, mono,
+  { apply encode_sizeof_le_of_infix, exact (l₀.drop_suffix i).is_infix, },
+  apply le_add_left, simp,
+  specialize hps ⟨S, a₀, l₀.take i⟩, simp at hps, refine hps.trans (monotone_polynomial_nat _ _),
+  ring_nf, simp, exact encode_sizeof_le_of_infix (l₀.take_prefix i).is_infix,
 end
-
-open polycodable (encode)
-variables {α β : Type*} [polycodable α] [polycodable β]
-def polycodable.decode [nonempty α] : ptree → α :=
-function.inv_fun (@encode α _)
-
-@[simp] lemma polycodable.decode_encode (x : α) : @polycodable.decode _ _ ⟨x⟩ (encode x) = x :=
-by { haveI : nonempty α := ⟨x⟩, exact function.left_inverse_inv_fun (function.embedding.injective _) x }
-
-lemma polytime_fun.polydecode [nonempty α] : polytime_fun (@polycodable.decode α _ _) :=
-begin
-  apply polytime_fun.decode,
-  convert_to polytime_fun (λ x : ptree, if x ∈ set.range (@encode α _) then x else (encode $ classical.arbitrary α)),
-  { ext x, split_ifs with h; simp [polycodable.decode],
-    { exact function.inv_fun_eq h }, { exact function.inv_fun_neg h, }, },
-  exact polytime_fun.ite (mem_poly α) polytime_fun.id (polytime_fun.const _),
-end
-
-lemma foldl_encode_comm (f : α → ptree → α) (acc : α) (l : list ptree) :
-  encode (l.foldl f acc) = l.foldl (λ a x, encode $ f (@polycodable.decode _ _ ⟨acc⟩ a) x) (encode acc) :=
-begin
-  induction l with hd tl ih generalizing acc, { simp, },
-  simp [ih],
-end
-
-lemma polytime_fun.foldl 
-  {f : α → β → ptree → β} {g : α → list ptree} {acc : α → β}
-  (hf : polytime_fun₃ f) (hg : polytime_fun g) (hacc : polytime_fun acc)
-  (hsize : polysize_fun (λ xls : list ptree × α × β, xls.1.foldl (f xls.2.1) xls.2.2)) :
-  polytime_fun (λ x, (g x).foldl (f x) (acc x)) :=
-begin
-  change polytime_fun (λ x, (@list.nil ptree, (g x).foldl (f x) (acc x)).snd),
-  apply polytime_fun.comp polytime_fun.prod_snd, swap, { apply_instance, /- For some reason Lean decided not to infer this instance -/ },
-  apply polytime_fun.decode, simp [function.comp],
-  sorry,
-  -- convert_to polytime_fun (λ x, (@list.nil ptree, (g x).foldl )) 
-end
-
-lemma list.all_eq_foldl {α : Type*} (P : α → bool) (l : list α) :
-  l.all P = l.foldl (λ r a, r && P a) tt :=
-begin
-  have : ∀ l : list α, l.foldl (λ r a, r && P a) ff = ff,
-  { clear l, intro l, induction l; simp [*], },
-  induction l with hd tl ih, { simp, }, cases h : P hd; simp [*],
-end
-
-lemma polytime_fun.list_all {P : ptree → bool} (hP : polytime_fun P) :
-  polytime_fun (λ l : list ptree, l.all P) :=
-begin
-  convert_to polytime_fun (λ l : list ptree, l.foldl (λ r a, r && P a) tt),
-  { ext l, exact list.all_eq_foldl _ _, },
-
-end
-
-#check bool.band_comm
-#check list.foldr_eq_of_comm'
-
--- local attribute [-instance] ptree_list_encoding_aux
 
 end list
