src/polycodable.lean
@@ -196,7 +196,15 @@ begin
   apply polytime_fun.ite, { simp, apply polytime_fun.comp, apply polytime_fun.is_none, exact hf, },
   apply polytime_fun.comp polytime_fun.encode hg, apply polytime_fun.comp polytime_fun.encode,
   apply polytime_fun.comp₂ hh polytime_fun.id, apply polytime_fun.comp polytime_fun.iget hf,
-end 
+end
+
+lemma polytime_fun.map {f : α → option β} {g : α → β → γ} (hf : polytime_fun f) (hg : polytime_fun₂ g) :
+  polytime_fun (λ x, (f x).map (g x)) :=
+begin
+  convert_to polytime_fun (λ x, (f x).elim none (λ r, some (g x r))),
+  { ext x : 1, cases (f x); simp, },
+  apply polytime_fun.option_elim hf, apply polytime_fun.const, simp only [polytime_fun₂, function.uncurry], apply polytime_fun.comp polytime_fun.some hg,
+end
 
 end option
 
